Games/gameLib/Conditioning.lean
@@ -1,0 +1,285 @@
+/-
+Copyright (c) 2024 Yves Jäckle. All rights reserved.
+Released under Apache 2.0 license as described in the file LICENSE.
+Author: Yves Jäckle.
+-/
+
+import Games.gameLib.Basic
+import Games.gameLib.Termination
+
+
+
+def Game_World_wDraw.world_after_fst {α β : Type u} (g : Game_World_wDraw α β)
+  (fst_act : β) : Game_World_wDraw α β := -- act not required to be legal
+  {g with init_game_state := g.fst_transition g.init_game_state [] fst_act }
+
+
+@[simp]
+lemma Game_World_wDraw.world_after_fst_init {α β : Type u} (g : Game_World_wDraw α β)
+  (fst_act : β) : (g.world_after_fst fst_act).init_game_state = g.fst_transition g.init_game_state [] fst_act :=
+  by rfl
+
+@[simp]
+lemma Game_World_wDraw.world_after_fst_fst_legal {α β : Type u} (g : Game_World_wDraw α β)
+  (fst_act : β) : (g.world_after_fst fst_act).fst_legal = g.fst_legal :=
+  by rfl
+
+@[simp]
+lemma Game_World_wDraw.world_after_fst_snd_legal {α β : Type u} (g : Game_World_wDraw α β)
+  (fst_act : β) : (g.world_after_fst fst_act).snd_legal = g.snd_legal :=
+  by rfl
+
+@[simp]
+lemma Game_World_wDraw.world_after_fst_fst_win_states {α β : Type u} (g : Game_World_wDraw α β)
+  (fst_act : β) : (g.world_after_fst fst_act).fst_win_states = g.fst_win_states :=
+  by rfl
+
+
+@[simp]
+lemma Game_World_wDraw.world_after_fst_snd_win_states {α β : Type u} (g : Game_World_wDraw α β)
+  (fst_act : β) : (g.world_after_fst fst_act).snd_win_states = g.snd_win_states :=
+  by rfl
+
+@[simp]
+lemma Game_World_wDraw.world_after_fst_draw_states {α β : Type u} (g : Game_World_wDraw α β)
+  (fst_act : β) : (g.world_after_fst fst_act).draw_states = g.draw_states :=
+  by rfl
+
+
+instance (l : List α): Decidable (l = []) :=
+  by
+  match l with
+  | [] => apply isTrue ; rfl
+  | x :: L => apply isFalse ; exact List.cons_ne_nil x L
+
+
+
+def fst_strat_deconditioned (s_strat : Strategy α β) (f_act : β) (g : Game_World_wDraw α β) : Strategy α β :=
+  (fun _ hist => if hist = [] then f_act else s_strat (g.world_after_fst f_act).init_game_state (hist.dropLast))
+
+def snd_strat_deconditioned (f_strat : Strategy α β) (f_act : β) (g : Game_World_wDraw α β) : Strategy α β :=
+  (fun _ hist => f_strat (g.world_after_fst f_act).init_game_state (hist.dropLast))
+
+
+lemma Game_World_wDraw.History_of_deconditioned
+  (g: Game_World_wDraw α β)
+  (fst_act: β)
+  (f_strat s_strat : Strategy α β)
+  (turn : ℕ):
+  let fst_strat := fst_strat_deconditioned s_strat fst_act g
+  let snd_strat := snd_strat_deconditioned f_strat fst_act g
+  History_on_turn g.init_game_state fst_strat snd_strat (turn + 1) =
+  (History_on_turn (g.world_after_fst fst_act).init_game_state f_strat s_strat turn) ++ [fst_act] :=
+  by
+  intro fst_strat snd_strat
+  induction' turn with t ih
+  · dsimp [History_on_turn, Turn_fst]
+    rw [if_pos (by decide), fst_strat_deconditioned, if_pos (by rfl)]
+  · dsimp only [History_on_turn] at *
+    by_cases q : Turn_fst (t+1)
+    · rw [Turn_fst_not_step] at q
+      rw [if_neg q] at *
+      rw [← Turn_fst_not_step] at q
+      rw [if_pos q, if_pos q] at *
+      rw [List.cons_append, ← ih]
+      congr
+      dsimp at ih
+      rw [← Game_World_wDraw.world_after_fst_init] at ih
+      rw [ih]
+      rw [snd_strat_deconditioned, List.dropLast_concat]
+    · rw [if_neg q, if_neg q] at *
+      rw [Turn_fst_not_step, not_not] at q
+      rw [if_pos q] at *
+      rw [fst_strat_deconditioned, snd_strat_deconditioned, if_neg (by apply List.cons_ne_nil)]
+      rw [List.cons_append, ← ih]
+      congr
+      dsimp [snd_strat_deconditioned] at ih
+      rw [← Game_World_wDraw.world_after_fst_init] at ih
+      rw [ih]
+      rw [List.dropLast_concat]
+
+
+def Game_World_wDraw.transition_blind_fst (g : Game_World_wDraw α β) : Prop :=
+  ∀ f_strat s_strat: Strategy α β, ∀ fst_act : β, g.fst_legal g.init_game_state [] fst_act →
+  let fst_strat := fst_strat_deconditioned s_strat fst_act g
+  let snd_strat := snd_strat_deconditioned f_strat fst_act g
+  ∀ turn : ℕ, ∀ act : β, g.snd_transition (g.world_after_fst fst_act).init_game_state (History_on_turn (g.world_after_fst fst_act).init_game_state f_strat s_strat turn) act
+    = g.fst_transition g.init_game_state (History_on_turn g.init_game_state fst_strat snd_strat (turn + 1)) act
+
+def Game_World_wDraw.transition_blind_snd (g : Game_World_wDraw α β) : Prop :=
+  ∀ f_strat s_strat: Strategy α β, ∀ fst_act : β, g.fst_legal g.init_game_state [] fst_act →
+  let fst_strat := fst_strat_deconditioned s_strat fst_act g
+  let snd_strat := snd_strat_deconditioned f_strat fst_act g
+  ∀ turn : ℕ, ∀ act : β, g.fst_transition (g.world_after_fst fst_act).init_game_state (History_on_turn (g.world_after_fst fst_act).init_game_state f_strat s_strat turn) act
+    = g.snd_transition g.init_game_state (History_on_turn g.init_game_state fst_strat snd_strat (turn + 1)) act
+
+
+def Game_World_wDraw.transition_blind (g : Game_World_wDraw α β) : Prop :=
+ g.transition_blind_fst ∧ g.transition_blind_snd
+
+
+def Game_World_wDraw.strong_transition_blind_fst (g : Game_World_wDraw α β) : Prop :=
+  ∀ fst_act : β, g.fst_legal g.init_game_state [] fst_act →
+  ∀ hist : List β, ∀ act : β, g.snd_transition (g.world_after_fst fst_act).init_game_state hist act
+    = g.fst_transition g.init_game_state (hist ++ [fst_act]) act
+
+def Game_World_wDraw.strong_transition_blind_snd (g : Game_World_wDraw α β) : Prop :=
+  ∀ fst_act : β, g.fst_legal g.init_game_state [] fst_act →
+  ∀ hist : List β, ∀ act : β, g.fst_transition (g.world_after_fst fst_act).init_game_state hist act
+    = g.snd_transition g.init_game_state (hist ++ [fst_act]) act
+
+
+def Game_World_wDraw.strong_transition_blind (g : Game_World_wDraw α β) : Prop :=
+ g.strong_transition_blind_fst ∧ g.strong_transition_blind_snd
+
+lemma Game_World_wDraw.strong_transition_blind_toWeak (g : Game_World_wDraw α β) :
+  g.strong_transition_blind → g.transition_blind :=
+  by
+  rintro ⟨f_strong, s_strong⟩
+  constructor
+  · intro f_strat s_strat f_act f_act_leg fst_strat snd_strat t act
+    rw [Game_World_wDraw.History_of_deconditioned]
+    apply f_strong
+    exact f_act_leg
+  · intro f_strat s_strat f_act f_act_leg fst_strat snd_strat t act
+    rw [Game_World_wDraw.History_of_deconditioned]
+    apply s_strong
+    exact f_act_leg
+
+
+
+def Game_World_wDraw.world_after_preHist {α β : Type u} (g : Game_World_wDraw α β)
+  (prehist : List β) : Game_World_wDraw α β := -- act not required to be legal
+  match prehist with
+  | [] => g
+  | last :: L => {g with init_game_state := g.fst_transition g.init_game_state L last}
+
+
+
+def Game_World_wDraw.hyper_transition_blind_fst (g : Game_World_wDraw α β) : Prop :=
+  ∀ prehist : List β, Hist_legal g.fst_legal g.snd_legal g.init_game_state prehist →
+  ∀ hist : List β, ∀ act : β, g.snd_transition (g.world_after_preHist prehist).init_game_state hist act
+    = g.fst_transition g.init_game_state (hist ++ prehist) act
+
+def Game_World_wDraw.hyper_transition_blind_snd (g : Game_World_wDraw α β) : Prop :=
+  ∀ prehist : List β, Hist_legal g.fst_legal g.snd_legal g.init_game_state prehist →
+  ∀ hist : List β, ∀ act : β, g.fst_transition (g.world_after_preHist prehist).init_game_state hist act
+    = g.snd_transition g.init_game_state (hist ++ prehist) act
+
+
+def Game_World_wDraw.hyper_transition_blind (g : Game_World_wDraw α β) : Prop :=
+ g.hyper_transition_blind_fst ∧ g.hyper_transition_blind_snd
+
+
+#exit
+
+lemma Game_World_wDraw.State_of_deconditioned
+  (g: Game_World_wDraw α β)
+  (tb : g.transition_blind)
+  (fst_act: β)
+  (fst_act_legal: g.fst_legal g.init_game_state [] fst_act)
+  (f_strat s_strat : Strategy α β)
+  (turn : ℕ):
+  let fst_strat := fst_strat_deconditioned s_strat fst_act g
+  let snd_strat := snd_strat_deconditioned f_strat fst_act g
+  g.state_on_turn fst_strat snd_strat (turn + 1) =
+  (g.world_after_fst fst_act).state_on_turn f_strat s_strat turn :=
+  by
+  intro fst_strat snd_strat
+  cases' turn with t
+  · dsimp [state_on_turn]
+    rw [if_pos (by decide)]
+    dsimp [history_on_turn, History_on_turn]
+    rw [fst_strat_deconditioned, if_pos (by rfl)]
+  · dsimp [state_on_turn]
+    by_cases q : Turn_fst (t + 1)
+    · rw [if_pos q]
+      rw [Turn_fst_not_step] at q
+      rw [if_neg q]
+      dsimp [history_on_turn]
+      have := g.History_of_deconditioned fst_act f_strat s_strat t
+      dsimp at this
+      rw [this]
+      rw [snd_strat_deconditioned, List.dropLast_concat]
+      rw [← this]
+      clear this
+      have := tb.2 f_strat s_strat fst_act fst_act_legal
+      dsimp at this
+      specialize this t (f_strat (world_after_fst g fst_act).toGame_World.init_game_state (History_on_turn (world_after_fst g fst_act).toGame_World.init_game_state f_strat s_strat t))
+      rw [← Game_World_wDraw.world_after_fst_init]
+      rw [← this]
+      clear this
+      rfl
+    · rw [Turn_not_fst_iff_snd, Turn_snd_fst_step] at q
+      rw [if_pos q]
+      dsimp [history_on_turn]
+      rw [← Turn_fst_step, Turn_fst_not_step] at q
+      rw [if_neg q]
+      rw [fst_strat_deconditioned, if_neg (by apply History_on_turn_nonempty_of_succ)]
+      have := g.History_of_deconditioned fst_act f_strat s_strat t
+      dsimp at this
+      rw [this]
+      rw [List.dropLast_concat]
+      rw [← this]
+      clear this
+      have := tb.1 f_strat s_strat fst_act fst_act_legal
+      dsimp at this
+      specialize this t (s_strat (world_after_fst g fst_act).toGame_World.init_game_state (History_on_turn (Game_World.fst_transition g.toGame_World g.init_game_state [] fst_act) f_strat s_strat t))
+      rw [← Game_World_wDraw.world_after_fst_init] at this
+      rw [← Game_World_wDraw.world_after_fst_init]
+      rw [← this]
+      clear this
+      rfl
+
+
+#exit
+
+lemma Game_World_wDraw.fst_legal_preconditioned'
+  (g: Game_World_wDraw α β)
+  (fst_act: β)
+  (fst_act_legal: g.fst_legal g.init_game_state [] fst_act)
+  (f_strat s_strat : Strategy α β)
+  (s_leg: Strategy_legal_snd (g.world_after_fst fst_act).init_game_state (fun x => (g.world_after_fst fst_act).snd_legal) f_strat s_strat)
+  (b : g.law_blind_fst')
+  :
+  let fst_strat : Strategy α β := (fun ini hist => if hist = [] then fst_act else s_strat (g.world_after_fst fst_act).init_game_state (hist.dropLast)) ;
+  let snd_strat : Strategy α β := (fun ini hist => f_strat (g.world_after_fst fst_act).init_game_state (hist.dropLast)) ;
+  Strategy_legal_fst g.init_game_state (fun x => g.fst_legal) fst_strat snd_strat :=
+  by
+  intro fst_strat snd_strat t tf
+  cases' t with t
+  · dsimp [History_on_turn]
+    rw [if_pos (by rfl)]
+    exact fst_act_legal
+  · rw [← b, Game_World_wDraw.History_of_preconditioned']
+    · dsimp [History_on_turn]
+      rw [if_neg (by apply List.append_ne_nil_of_ne_nil_right ; exact List.cons_ne_nil fst_act [])]
+      rw [List.dropLast_concat]
+      apply s_leg
+      rw [Turn_snd_fst_step]
+      exact tf
+    · exact fst_act_legal
+
+
+lemma Game_World_wDraw.snd_legal_preconditioned'
+  (g: Game_World_wDraw α β)
+  (fst_act: β)
+  (fst_act_legal: g.fst_legal g.init_game_state [] fst_act)
+  (f_strat s_strat : Strategy α β)
+  (f_leg: Strategy_legal_fst (g.world_after_fst fst_act).init_game_state (fun x => (g.world_after_fst fst_act).fst_legal) f_strat s_strat)
+  (b : g.law_blind_snd')
+  :
+  let fst_strat : Strategy α β := (fun ini hist => if hist = [] then fst_act else s_strat (g.world_after_fst fst_act).init_game_state (hist.dropLast)) ;
+  let snd_strat : Strategy α β := (fun ini hist => f_strat (g.world_after_fst fst_act).init_game_state (hist.dropLast)) ;
+  Strategy_legal_snd g.init_game_state (fun x => g.snd_legal) fst_strat snd_strat :=
+  by
+  intro fst_strat snd_strat t tf
+  cases' t with t
+  · contradiction
+  · rw [← b, Game_World_wDraw.History_of_preconditioned']
+    · dsimp [History_on_turn]
+      rw [List.dropLast_concat]
+      apply f_leg
+      rw [Turn_fst_snd_step]
+      exact tf
+    · exact fst_act_legal
